More automation and top-level theorems

src/AttarchProperties.v
@@ -10,10 +10,6 @@ Open Scope tprop_scope.
 Open Scope env_scope.
 
 
-Ltac star_notation := 
-  repeat change (clos_refl_trans_n1 _ ?R) with (R^*) in *.
-
-
 Definition diverged : tprop attarch_state :=
   <[λ '(l, _), l = attarch_bot]>.
 
@@ -31,19 +27,16 @@ Proof.
   intros s0 s0_init.
   apply star__AG.
   intros s Hstar.
-  induct! Hstar; star_notation.
+  induct! Hstar; star_notation; [|attarch_step_inv]; try rw_solver.
   - destruct or s0_init;
     rewritec s0_init;
     follows tentails!.
-  - invc H; try rw_solver.
-    + invc H; try rw_solver.
-      tentails! in *.
-      intros .
-      destruct H5 as (acc & a & lookup & Hacc & ->).
-      unbox a.
-      simpl_rws.
-      follows eapply IHHstar.
-    + invc H; invc H0; rw_solver.
+  - tentails! in *.
+    intros .
+    destruct H5 as (acc & a & lookup & Hacc & ->).
+    unbox a.
+    simpl_rws.
+    follows eapply IHHstar.
 Qed.
 
 
@@ -52,10 +45,6 @@ Definition useram_key_secure : tprop attarch_state := <[λ '(_, Γ),
     read Γ c "useram_key" good_useram_key -> 
     c = "useram"
 ]>.
-
-(* Definition useram_key_released : tprop attarch_state := <[λ '(l, _),
-  exists vl, l = sel4_run platam_listen vl
-]>. *)
 
 Definition useram_key_released : tprop attarch_state := <[λ '(l, _),
   exists pl ul,
@@ -87,21 +76,123 @@ Proof.
     rw_solver.
   - intros * Hstar Hs' * H.
     destruct Hs' as [Hs'l Hs'r].
-    invc H.
-    + left. rw_solver with find inject.
-    + left. rw_solver with find inject.
-    + invc H; left; rw_solver.
-    + invc H; invc H0; try (left + right; rw_solver).
-      left.
-      tentails! in *.
-      destruct H as (acc & V & v & lookup & ->).
-      intros acc' key Hacc'.
-      inject Hacc'.
-      eapply Hs'l.
-      eassumption.
-    + left. rw_solver.
+    attarch_step_inv; solve[left + right; rw_solver!].
 Qed.
+
+
+Definition os_corrupted : tprop attarch_state := <[λ '(_, Γ),
+  exists acc, Γ "good_os" = Some (acc, box false)
+]>.
+
+Theorem os_corrupted_permanent' : forall pl vl Γ,
+  attarch_trans @(sel4_run pl vl, Γ) ⊨ os_corrupted --> AG os_corrupted.
+Proof using.
+  intros *.
+  tintro H.
+  tentails! in H.
+  destruct H as [acc lookup].
+  apply star__AG.
+  intros * Hstar.
+  induct! Hstar; star_notation.
+  - follows tentails!.
+  - attarch_step_inv; 
+      try (invc Hstar; find (fun H => solve[inversion H]));
+      rw_solver!.
+Qed.
+
+Theorem os_corrupted_permanent : forall s0,
+  is_init_attarch_state s0 ->
+  attarch_trans @s0 ⊨ AG (os_corrupted --> AG os_corrupted).
+Proof using.
+  intros s0 Hs0.
+  apply star__AG.
+  intros * Hstar.
+  induct! Hstar; star_notation.
+  - tintro.
+    exfalso.
+    destruct or Hs0; rewrite Hs0 in *;
+      follows tentails! in *.
+  - attarch_step_inv; try apply os_corrupted_permanent'.
+    clear.
+    tintro H.
+    apply star__AG.
+    intros * Hstar.
+    induct! Hstar; star_notation; [|attarch_step_inv]; 
+      try (invc Hstar; find (fun H => solve[inversion H]));
+      rw_solver!.
+Qed.
+
+
+Definition deep_attesting : tprop attarch_state := <[λ '(l, _),
+  l = sel4_run platam_deep_attest (vm_run useram_deep_attest)
+]>.
+
+Definition starting_shallow_attest : tprop attarch_state := <[λ '(l, _),
+  exists pl, l = sel4_run pl (vm_run useram_shallow_attest)
+]>.
+
+Definition finished_shallow_attest : tprop attarch_state := <[λ '(l, _),
+  exists pl, l = sel4_run pl (vm_run useram_listen)
+]>.
+
+Definition trustworthy_attest_result : tprop attarch_state := <[λ '(_, Γ),
+  forall acc acc' (b: bool),
+    Γ "shallow_attest_result" = Some (acc, box b) ->
+    Γ "good_target" = Some (acc', box b)
+]>.
+
+Theorem deep_attest_corruption_window_aux : forall Γ,
+  attarch_trans @(sel4_run platam_deep_attest (vm_run useram_listen), Γ) ⊨
+    A[(starting_shallow_attest -->
+      A[(finished_shallow_attest --> trustworthy_attest_result) W os_corrupted])
+    W os_corrupted].
+Proof using.
+  intros *.
+  apply AW_intro_weak.
+  - left. rw_solver.
+  - intros * Hstar [Htrust Hnot_corrupt] * H.
+    invc H; try (left; rw_solver).
+    + invc H.
+      * left.
+        tintros.
+        tentails! in *.
+        destruct H as [? H].
+        inject H.
  
+
+  intros *.
+  apply AW_intro; split.
+  - left. rw_solver.
+  (* - intros * [Htrust Hnot_corrupt] * Hstep. *)
+  - intros * H * Hstep.
+    invc Hstep; try (left; rw_solver).
+    + invc H0.
+      * 
+
+
+Theorem deep_attest_corruption_window :
+  attarch_trans @attarch_good_init_state ⊨
+    AG (deep_attesting -->
+      A[(starting_shallow_attest -->
+        A[(finished_shallow_attest --> trustworthy_attest_result) W os_corrupted])
+      W os_corrupted]).
+Proof using.
+  intros.
+
+(* ⊨ os_corrupted --> AG os_corrupted *)
+
+(* ⊨ AG (deep_attesting --> A[(ul = useram_shallow_attest) --> A[(ul = useram_listen --> good_meas_value) W mal] W mal]) *)
+
+(* Definition foo : tprop attarch_state := <[λ '(l, Γ),
+]>. *)
+
+
+(* ⊨ AG (deep_attest --> A[trustworthy_attest W os_corruption]) *)
+
+
+(* ⊨ A[(os_corruption --> EF detect_corruption) W diverged] *)
+(* ⊨ A[(useram_leak --> EF detect_leak) W diverged] *)
+
 
 Close Scope tprop_scope.
 Close Scope string_scope.
